Auxiliary/Interview.dfy
@@ -35,6 +35,7 @@ type Interview< T(==) > {
     ensures e.Valid()
     ensures e.Model() == if b then Model().True else Model().False
     ensures e.Questions() == Questions() - {Model().Key}
+    ensures |e.Questions()| == |Questions()| - 1
     ensures e.Candidates() == (set cand:candidate | cand in Candidates() && cand[Model().Key] == b :: cand)
     ensures counter_out == counter_in + UBSize()
   
