Auxiliary/Lemmas.dfy
@@ -7,6 +7,12 @@ lemma mult_preserves_order(a:int, b:int, a':int, b':int)
   ensures a*b <= a'*b'
 {}
 
+lemma mult_preserves_strict_order(a:int, b:int, a':int, b':int)
+  requires 0 <= a < a'
+  requires 0 < b <= b'
+  ensures a*b < a'*b'
+{}
+
 lemma associativity(a:int, b:int, c:int)
   ensures (a*b)*c == a*(b*c)
 {}
